theories/Pre_orders/Must/Must.v
@@ -404,7 +404,7 @@ Notation "p ≼₁ q" := (bhv_pre_cond1 p q) (at level 70).
 (********************************** Infinite Branching Lts to Finite Branching Lts **********************)
 Class AbsAction `{H : ExtAction A} {E FinA : Type} (LtsE : @gLts E A H) (Φ : A → FinA) :=
   MkAbsAction {
-    abstraction_test_spec μ μ' e : (Φ μ) = (Φ μ') -> ¬ e ↛[ μ ] -> ¬ e ↛[ μ' ]
+    abstraction_test_spec μ μ' e : blocking μ -> blocking μ' -> (Φ μ) = (Φ μ') -> ¬ e ↛[ μ ] -> ¬ e ↛[ μ' ]
   }.
 
 
@@ -419,7 +419,11 @@ Class PreExtAction `{H : ExtAction A} {P FinA: Type} `{Countable PreAct}
             -> ∃ μ', μ' ∈ co_actions_of p /\ pre_μ = (Φ μ');
 
       pre_co_actions_of : P -> gset PreAct;
-      preactions_of_spec (pre_μ : FinA) (p : P) : pre_μ ∈ (pre_co_actions_of_fin p) <-> (𝝳 pre_μ) ∈ (pre_co_actions_of p);
+      preactions_of_spec1 (pre_μ : FinA) (p : P) : pre_μ ∈ (pre_co_actions_of_fin p) 
+        -> (𝝳 pre_μ) ∈ (pre_co_actions_of p);
+      preactions_of_spec2 (pre_pre_μ : PreAct) (pre_μ : FinA) (p : P) : 
+      (𝝳 pre_μ) = pre_pre_μ -> pre_pre_μ ∈ (pre_co_actions_of p) 
+        -> pre_μ ∈ (pre_co_actions_of_fin p);
   }.
 
 Definition bhv_pre_cond2 `{
